Progress on the IL2 verification.
Showed that the closures w/o cenv behave the same as the ones with, at
the expression level. The declaration level is still to do.

compiler/proofs/toIntLang2ProofScript.sml
@@ -2,6 +2,7 @@ open preamble;
 open alistTheory optionTheory rich_listTheory;
 open miscTheory;
 open astTheory;
+open semanticPrimitivesTheory;
 open libTheory;
 open libPropsTheory;
 open intLang1Theory;
@@ -10,6 +11,20 @@ open toIntLang1ProofTheory;
 open evalPropsTheory;
 
 val _ = new_theory "toIntLang2Proof";
+
+val fmap_inverse_def = Define `
+fmap_inverse m1 m2 =
+  !k. k ∈ FDOM m1 ⇒ ?v. FLOOKUP m1 k = SOME v ∧ FLOOKUP m2 v = SOME k`;
+
+val same_tid_diff_ctor = Q.prove (
+`!cn1 cn2 t1 t2.
+  same_tid t1 t2 ∧ ~same_ctor (cn1, t1) (cn2, t2)
+  ⇒
+  (cn1 ≠ cn2) ∨ (cn1 = cn2 ∧ ?mn1 mn2. t1 = TypeExn mn1 ∧ t2 = TypeExn mn2 ∧ mn1 ≠ mn2)`,
+rw [] >>
+cases_on `t1` >>
+cases_on `t2` >>
+fs [same_tid_def, same_ctor_def]);
 
 fun register name def ind =
   let val _ = save_thm (name ^ "_def", def);
@@ -52,111 +67,1027 @@ val (do_eq_i2_def, do_eq_i2_ind) =
                                         | INR (xs,ys) => v_i23_size xs)`);
 val _ = register "do_eq_i2" do_eq_i2_def do_eq_i2_ind;
 
+val build_rec_env_i2_help_lem = Q.prove (
+`∀funs env funs'.
+FOLDR (λ(f,x,e) env'. bind f (Recclosure_i2 env funs' f) env') env' funs =
+merge (MAP (λ(fn,n,e). (fn, Recclosure_i2 env funs' fn)) funs) env'`,
+Induct >>
+rw [merge_def, bind_def] >>
+PairCases_on `h` >>
+rw []);
+
+val build_rec_env_i2_merge = Q.store_thm ("build_rec_env_i2_merge",
+`∀funs funs' env env'.
+  build_rec_env_i2 funs env env' =
+  merge (MAP (λ(fn,n,e). (fn, Recclosure_i2 env funs fn)) funs) env'`,
+rw [build_rec_env_i2_def, build_rec_env_i2_help_lem]);
+
+val funs_to_i2_map = Q.prove (
+`!funs.
+  funs_to_i2 cenv funs = MAP (\(f,x,e). (f,x,exp_to_i2 cenv e)) funs`,
+ induct_on `funs` >>
+ rw [exp_to_i2_def] >>
+ PairCases_on `h` >>
+ rw [exp_to_i2_def]);
+
 val lookup_type_tag_def = Define `
 (lookup_type_tag NONE cenv = SOME tuple_tag) ∧
 (lookup_type_tag (SOME cn) (next,env,type_cenv,inv) = FLOOKUP type_cenv cn)`;
 
-val v_to_i2_def = tDefine "v_to_i2" `
- (v_to_i2 cenv (Litv_i1 l) = SOME (Litv_i2 l)) ∧
- (v_to_i2 cenv (Conv_i1 cn vs) =
-   case lookup_type_tag cn cenv of
-        NONE => NONE
-      | SOME tag => 
-          case vs_to_i2 cenv vs of
-               NONE => NONE
-             | SOME vs' => SOME (Conv_i2 tag vs')) ∧
- (v_to_i2 cenv (Closure_i1 (cenv',env) x e) =
-   case env_to_i2 cenv env of
-        NONE => NONE
-      | SOME env' => 
-          SOME (Closure_i2 env' x (exp_to_i2 cenv e))) ∧
- (v_to_i2 cenv (Recclosure_i1 (cenv',env) funs x) =
-   case env_to_i2 cenv env of
-        NONE => NONE
-      | SOME env' => 
-          SOME (Recclosure_i2 env' (funs_to_i2 cenv funs) x)) ∧
- (v_to_i2 cenv (Loc_i1 l) = SOME (Loc_i2 l)) ∧
- (vs_to_i2 cenv [] = SOME []) ∧
- (vs_to_i2 cenv (v::vs) =
-   case v_to_i2 cenv v of
-      NONE => NONE
-    | SOME v' =>
-        case vs_to_i2 cenv vs of
-             NONE => NONE
-           | SOME vs' => SOME (v'::vs')) ∧
- (env_to_i2 cenv [] = SOME []) ∧
- (env_to_i2 cenv ((x,v)::env) =
-   case v_to_i2 cenv v of
-      NONE => NONE
-    | SOME v' =>
-        case env_to_i2 cenv env of
-             NONE => NONE
-           | SOME env' => SOME ((x,v')::env'))`
-cheat;
-
-val fmap_inverse_def = Define `
-fmap_inverse m1 m2 =
-  !k. k ∈ FDOM m1 ⇒ ?v. FLOOKUP m1 k = SOME v ∧ FLOOKUP m2 v = SOME k`;
+val has_exns_def = Define `
+has_exns (cenv, clengths) ⇔
+  FLOOKUP clengths ("Bind", TypeExn NONE) = SOME (0:num) ∧
+  FLOOKUP clengths ("Div", TypeExn NONE) = SOME 0 ∧
+  FLOOKUP clengths ("Eq", TypeExn NONE) = SOME 0 ∧
+  FLOOKUP cenv ("Bind", TypeExn NONE) = SOME bind_tag ∧
+  FLOOKUP cenv ("Div", TypeExn NONE) = SOME div_tag ∧
+  FLOOKUP cenv ("Eq", TypeExn NONE) = SOME eq_tag`;
 
 val cenv_inv_def = Define `
-cenv_inv cenv (next,lex_cenv,type_cenv,inverse_cenv) ⇔
-  (!id n. FLOOKUP lex_cenv id = SOME n ⇒ 
-          ?l t. lookup_con_id id cenv = SOME (l,t) ∧
-                FLOOKUP type_cenv (id_to_n id,t) = SOME n) ∧
-  (fmap_inverse type_cenv inverse_cenv) ∧
-  (fmap_inverse inverse_cenv type_cenv)`;
+cenv_inv (cenv:envC) ((next, lex_cenv, type_cenv, inverse_cenv):cenv_mapping) (clengths:(conN#tid_or_exn)|-> num) ⇔
+  (!cn num_args t.
+    lookup_con_id cn cenv = SOME (num_args, t)
+    ⇒
+    FLOOKUP clengths (id_to_n cn,t) = SOME num_args ∧
+    ?tag.
+      FLOOKUP lex_cenv cn = SOME tag ∧
+      FLOOKUP type_cenv (id_to_n cn, t) = SOME tag) ∧
+  (!cn. FLOOKUP type_cenv cn ≠ SOME tuple_tag) ∧
+  has_exns (type_cenv,clengths) ∧
+  (!t1 t2 tag cn cn'.
+     (* Comment out same_tid because we're not using separate tag spaces per type *)
+     (* same_tid t1 t2 ∧ *)
+     FLOOKUP type_cenv (cn,t1) = SOME tag ∧
+     FLOOKUP type_cenv (cn',t2) = SOME tag
+     ⇒
+     cn = cn' ∧ t1 = t2)`;
+
+val (v_to_i2_rules, v_to_i2_ind, v_to_i2_cases) = Hol_reln `
+(!cenv lit.
+  v_to_i2 cenv (Litv_i1 lit) (Litv_i2 lit)) ∧
+(!cenv vs vs'.
+  vs_to_i2 cenv vs vs'
+  ⇒ 
+  v_to_i2 cenv (Conv_i1 NONE vs) (Conv_i2 tuple_tag vs')) ∧
+(!cenv clengths cn tn tag vs vs'.
+  FLOOKUP cenv (cn,tn) = SOME tag ∧
+  FLOOKUP clengths (cn,tn) = SOME (LENGTH vs) ∧
+  vs_to_i2 (cenv,clengths) vs vs'
+  ⇒ 
+  v_to_i2 (cenv,clengths) (Conv_i1 (SOME (cn,tn)) vs) (Conv_i2 tag vs')) ∧
+(!cenv env x e env_i2 envC next lex_cenv inverse_cenv.
+  env_to_i2 (cenv,clengths) env env_i2 ∧
+  cenv_inv envC (next, lex_cenv, cenv, inverse_cenv) clengths
+  ⇒ 
+  v_to_i2 (cenv,clengths) (Closure_i1 (envC,env) x e) (Closure_i2 env_i2 x (exp_to_i2 (next, lex_cenv, cenv, inverse_cenv) e))) ∧ 
+(!cenv env funs x envC env_i2 next lex_cenv inverse_cenv.
+  env_to_i2 (cenv,clengths) env env_i2 ∧
+  cenv_inv envC (next, lex_cenv, cenv, inverse_cenv) clengths
+  ⇒ 
+  v_to_i2 (cenv,clengths) (Recclosure_i1 (envC,env) funs x) (Recclosure_i2 env_i2 (funs_to_i2 (next, lex_cenv, cenv, inverse_cenv) funs) x)) ∧
+(!cenv loc.
+  v_to_i2 cenv (Loc_i1 loc) (Loc_i2 loc)) ∧
+(!cenv.
+  vs_to_i2 cenv [] []) ∧
+(!cenv v vs v' vs'.
+  v_to_i2 cenv v v' ∧
+  vs_to_i2 cenv vs vs'
+  ⇒
+  vs_to_i2 cenv (v::vs) (v'::vs')) ∧
+(!cenv.
+  env_to_i2 cenv [] []) ∧
+(!cenv x v env env' v'. 
+  env_to_i2 cenv env env' ∧
+  v_to_i2 cenv v v'
+  ⇒ 
+  env_to_i2 cenv ((x,v)::env) ((x,v')::env'))`;
+
+val v_to_i2_eqns = Q.prove (
+`(!cenv l v.
+  v_to_i2 cenv (Litv_i1 l) v ⇔ 
+    (v = Litv_i2 l)) ∧
+ (!cenv cn vs v.
+  v_to_i2 cenv (Conv_i1 cn vs) v ⇔ 
+    (?vs' tag cenv' clengths.
+       vs_to_i2 cenv vs vs' ∧ (v = Conv_i2 tag vs') ∧
+       (cn = NONE ∧ tag = tuple_tag ∨
+        ?cenv' clengths cn' tn.
+          cenv = (cenv',clengths) ∧
+          FLOOKUP cenv' (cn',tn) = SOME tag ∧
+          FLOOKUP clengths (cn',tn) = SOME (LENGTH vs) ∧
+          cn = SOME (cn',tn) ∧ FLOOKUP cenv' (cn', tn) = SOME tag))) ∧
+ (!cenv l v.
+  v_to_i2 cenv (Loc_i1 l) v ⇔ 
+    (v = Loc_i2 l)) ∧
+ (!cenv vs.
+  vs_to_i2 cenv [] vs ⇔ 
+    (vs = [])) ∧
+ (!cenv l v vs vs'.
+  vs_to_i2 cenv (v::vs) vs' ⇔ 
+    ?v' vs''. v_to_i2 cenv v v' ∧ vs_to_i2 cenv vs vs'' ∧ vs' = v'::vs'') ∧
+ (!cenv env'.
+  env_to_i2 cenv [] env' ⇔
+    env' = []) ∧
+ (!cenv x v env env'.
+  env_to_i2 cenv ((x,v)::env) env' ⇔
+    ?v' env''. v_to_i2 cenv v v' ∧ env_to_i2 cenv env env'' ∧ env' = ((x,v')::env''))`,
+rw [] >>
+rw [Once v_to_i2_cases] >>
+metis_tac []);
+
+val cenv_mapping_weak_def = Define `
+
+
+val v_to_i2_weakening = Q.prove (
+`(!cenv v v_i2.
+  v_to_i2 cenv v v_i2
+  ⇒
+  ∀cenv'. v_to_i2 cenv v v_i2) ∧
+ (!cenv vs vs_i2.
+  vs_to_i2 cenv vs vs_i2
+  ⇒
+  !cenv'. vs_to_i2 cenv') vs vs_i2) ∧
+ (!cenv env env_i2.
+  env_to_i2 cenv env env_i2
+  ⇒
+  !cenv'. env_to_i2 cenv' env env_i2)`,
+
+
+
+val (result_to_i2_rules, result_to_i2_ind, result_to_i2_cases) = Hol_reln `
+(∀genv v v'. 
+  f genv v v'
+  ⇒
+  result_to_i2 f genv (Rval v) (Rval v')) ∧
+(∀genv v v'. 
+  v_to_i2 genv v v'
+  ⇒
+  result_to_i2 f genv (Rerr (Rraise v)) (Rerr (Rraise v'))) ∧
+(!genv.
+  result_to_i2 f genv (Rerr Rtimeout_error) (Rerr Rtimeout_error)) ∧
+(!genv.
+  result_to_i2 f genv (Rerr Rtype_error) (Rerr Rtype_error))`;
+
+val result_to_i2_eqns = Q.prove (
+`(!genv v r.
+  result_to_i2 f genv (Rval v) r ⇔ 
+    ?v'. f genv v v' ∧ r = Rval v') ∧
+ (!genv v r.
+  result_to_i2 f genv (Rerr (Rraise v)) r ⇔ 
+    ?v'. v_to_i2 genv v v' ∧ r = Rerr (Rraise v')) ∧
+ (!genv v r.
+  result_to_i2 f genv (Rerr Rtimeout_error) r ⇔ 
+    r = Rerr Rtimeout_error) ∧
+ (!genv v r.
+  result_to_i2 f genv (Rerr Rtype_error) r ⇔ 
+    r = Rerr Rtype_error)`,
+rw [result_to_i2_cases] >>
+metis_tac []);
+
+val (s_to_i2'_rules, s_to_i2'_ind, s_to_i2'_cases) = Hol_reln `
+(!genv s s'.
+  vs_to_i2 genv s s'
+  ⇒
+  s_to_i2' genv s s')`;
+
+val (s_to_i2_rules, s_to_i2_ind, s_to_i2_cases) = Hol_reln `
+(!genv c s s'.
+  s_to_i2' genv s s'
+  ⇒
+  s_to_i2 genv (c,s) (c,s'))`;
 
 val length_vs_to_i2 = Q.prove (
 `!vs cenv vs'. 
-  vs_to_i2 cenv vs = SOME vs'
+  vs_to_i2 cenv vs vs'
   ⇒
   LENGTH vs = LENGTH vs'`,
  induct_on `vs` >>
- rw [v_to_i2_def] >>
- fs [] >>
- every_case_tac >>
- fs [] >>
+ rw [v_to_i2_eqns] >>
  rw [] >>
  metis_tac []);
 
+val length_evaluate_list_i2 = Q.prove (
+`!b env s cenv es s' vs.
+  evaluate_list_i2 b env s (exps_to_i2 cenv es) (s', Rval vs)
+  ⇒
+  LENGTH es = LENGTH vs`,
+ induct_on `es` >>
+ rw [exp_to_i2_def] >>
+ cases_on `vs` >>
+ pop_assum (mp_tac o SIMP_RULE (srw_ss()) [Once evaluate_i2_cases]) >>
+ rw [] >>
+ metis_tac []);
+
+val env_to_i2_el = Q.prove (
+`!cenv env env_i2. 
+  env_to_i2 cenv env env_i2 ⇔ 
+  LENGTH env = LENGTH env_i2 ∧ !n. n < LENGTH env ⇒ (FST (EL n env) = FST (EL n env_i2)) ∧ v_to_i2 cenv (SND (EL n env)) (SND (EL n env_i2))`,
+ induct_on `env` >>
+ rw [v_to_i2_eqns]
+ >- (cases_on `env_i2` >>
+     fs []) >>
+ PairCases_on `h` >>
+ rw [v_to_i2_eqns] >>
+ eq_tac >>
+ rw [] >>
+ rw []
+ >- (cases_on `n` >>
+     fs [])
+ >- (cases_on `n` >>
+     fs [])
+ >- (cases_on `env_i2` >>
+     fs [] >>
+     FIRST_ASSUM (qspecl_then [`0`] mp_tac) >>
+     SIMP_TAC (srw_ss()) [] >>
+     rw [] >>
+     qexists_tac `SND h` >>
+     rw [] >>
+     FIRST_X_ASSUM (qspecl_then [`SUC n`] mp_tac) >>
+     rw []));
+
+
+val vs_to_i2_lupdate = Q.prove (
+`!cenv v n s v_i2 n s_i2.
+  vs_to_i2 cenv s s_i2 ∧
+  v_to_i2 cenv v v_i2
+  ⇒
+  vs_to_i2 cenv (LUPDATE v n s) (LUPDATE v_i2 n s_i2)`,
+ induct_on `n` >>
+ rw [v_to_i2_eqns, LUPDATE_def] >>
+ cases_on `s` >>
+ fs [v_to_i2_eqns, LUPDATE_def]);
+
 val match_result_to_i2_def = Define 
 `(match_result_to_i2 cenv (Match env) (Match env_i2) ⇔ 
-   env_to_i2 cenv env = SOME env_i2) ∧
+   env_to_i2 cenv env env_i2) ∧
  (match_result_to_i2 cenv No_match No_match = T) ∧
  (match_result_to_i2 cenv Match_type_error Match_type_error = T) ∧
  (match_result_to_i2 cenv _ _ = F)`;
 
+val store_lookup_vs_to_i2 = Q.prove (
+`!cenv vs vs_i2 v v_i2 n.
+  vs_to_i2 cenv vs vs_i2 ∧
+  store_lookup n vs = SOME v ∧
+  store_lookup n vs_i2 = SOME v_i2
+  ⇒
+  v_to_i2 cenv v v_i2`,
+ induct_on `vs` >>
+ rw [v_to_i2_eqns] >>
+ fs [store_lookup_def] >>
+ cases_on `n` >>
+ fs [] >>
+ metis_tac []);
+
+val store_lookup_vs_to_i2_2 = Q.prove (
+`!cenv vs vs_i2 v v_i2 n.
+  vs_to_i2 cenv vs vs_i2 ∧
+  store_lookup n vs = SOME v
+  ⇒
+  ?v'. store_lookup n vs_i2 = SOME v'`,
+ induct_on `vs` >>
+ rw [v_to_i2_eqns] >>
+ fs [store_lookup_def] >>
+ cases_on `n` >>
+ fs [] >>
+ metis_tac []);
+
+val pat_bindings_i2_accum = Q.store_thm ("pat_bindings_ai2_ccum",
+`(!p acc. pat_bindings_i2 p acc = pat_bindings_i2 p [] ++ acc) ∧
+ (!ps acc. pats_bindings_i2 ps acc = pats_bindings_i2 ps [] ++ acc)`,
+ Induct >>
+ rw []
+ >- rw [pat_bindings_i2_def]
+ >- rw [pat_bindings_i2_def]
+ >- metis_tac [APPEND_ASSOC, pat_bindings_i2_def]
+ >- metis_tac [APPEND_ASSOC, pat_bindings_i2_def]
+ >- rw [pat_bindings_i2_def]
+ >- metis_tac [APPEND_ASSOC, pat_bindings_i2_def]);
+
+val pat_bindings_to_i2 = Q.prove (
+`!cenv p x. pat_bindings_i2 (pat_to_i2 cenv p) x = pat_bindings p x`,
+ ho_match_mp_tac pat_to_i2_ind >>
+ rw [pat_bindings_def, pat_bindings_i2_def, pat_to_i2_def] >>
+ induct_on `ps` >>
+ rw [] >>
+ fs [pat_bindings_def, pat_bindings_i2_def, pat_to_i2_def] >>
+ metis_tac [APPEND_11, pat_bindings_accum, pat_bindings_i2_accum]);
+
 val pmatch_to_i2_correct = Q.prove (
-`(!cenv s p v env r env_i2 s_i2 v_i2 cenv'.
+`(!envC s p v env r env_i2 s_i2 v_i2 next lex_cenv cenv inverse_cenv clengths.
   r ≠ Match_type_error ∧
-  cenv_inv cenv cenv' ∧
-  pmatch_i1 cenv s p v env = r ∧
-  s_to_i2' cenv' s s_i2 ∧
-  v_to_i2 cenv' v = SOME v_i2 ∧
-  env_to_i2 cenv' env = SOME env_i2
+  cenv_inv envC (next,lex_cenv,cenv,inverse_cenv) clengths ∧
+  pmatch_i1 envC s p v env = r ∧
+  s_to_i2' (cenv,clengths) s s_i2 ∧
+  v_to_i2 (cenv,clengths) v v_i2 ∧
+  env_to_i2 (cenv,clengths) env env_i2
   ⇒
   ?r_i2.
-    pmatch_i2 s_i2 (pat_to_i2 cenv' p) v_i2 env_i2 = r_i2 ∧
-    match_result_to_i2 cenv' r r_i2) ∧
- (!cenv s ps vs env r env_i2 s_i2 vs_i2 cenv'.
+    pmatch_i2 s_i2 (pat_to_i2 (next,lex_cenv,cenv,inverse_cenv) p) v_i2 env_i2 = r_i2 ∧
+    match_result_to_i2 (cenv,clengths) r r_i2) ∧
+ (!envC s ps vs env r env_i2 s_i2 vs_i2 next lex_cenv cenv inverse_cenv clengths.
   r ≠ Match_type_error ∧
-  cenv_inv cenv cenv' ∧
-  pmatch_list_i1 cenv s ps vs env = r ∧
-  s_to_i2' cenv' s s_i2 ∧
-  vs_to_i2 cenv' vs = SOME vs_i2 ∧
-  env_to_i2 cenv' env = SOME env_i2
+  cenv_inv envC (next,lex_cenv,cenv,inverse_cenv) clengths ∧
+  pmatch_list_i1 envC s ps vs env = r ∧
+  s_to_i2' (cenv,clengths) s s_i2 ∧
+  vs_to_i2 (cenv,clengths) vs vs_i2 ∧
+  env_to_i2 (cenv,clengths) env env_i2
   ⇒
   ?r_i2.
-    pmatch_list_i2 s_i2 (MAP (pat_to_i2 cenv') ps) vs_i2 env_i2 = r_i2 ∧
-    match_result_to_i2 cenv' r r_i2)`,
-
+    pmatch_list_i2 s_i2 (MAP (pat_to_i2 (next,lex_cenv,cenv,inverse_cenv)) ps) vs_i2 env_i2 = r_i2 ∧
+    match_result_to_i2 (cenv,clengths) r r_i2)`,
  ho_match_mp_tac pmatch_i1_ind >>
- rw [pmatch_i1_def, pmatch_i2_def] >>
- fs [match_result_to_i2_def, bind_def, pmatch_i2_def, v_to_i2_def, pat_to_i2_def] >>
- rw [pmatch_i2_def, match_result_to_i2_def] >>
+ rw [pmatch_i1_def, pmatch_i2_def, pat_to_i2_def, match_result_to_i2_def] >>
+ fs [match_result_to_i2_def, bind_def, v_to_i2_eqns] >>
+ rw [pmatch_i2_def, match_result_to_i2_def]
+ >- (cases_on `lookup_con_id n envC` >>
+     fs [] >>
+     every_case_tac >>
+     fs [] 
+     >- metis_tac [] >>
+     fs [lookup_tag_def, cenv_inv_def] >>
+     res_tac >>
+     fs [] >>
+     rw [] >>
+     imp_res_tac same_tid_diff_ctor >>
+     rw [] >>
+     metis_tac [tid_or_exn_11])
+ >- (cases_on `lookup_con_id n envC` >>
+     fs [] >>
+     every_case_tac >>
+     fs [] >> 
+     rw []
+     >- metis_tac [length_vs_to_i2, cenv_inv_def, SOME_11, same_ctor_and_same_tid] >>
+     fs [lookup_tag_def, cenv_inv_def] >>
+     res_tac >>
+     fs [] >>
+     rw [] >>
+     imp_res_tac same_tid_diff_ctor >>
+     rw [] >>
+     metis_tac [tid_or_exn_11])
+ >- (cases_on `lookup_con_id n envC` >>
+     fs [] >>
+     every_case_tac >>
+     fs [lookup_tag_def, cenv_inv_def] >>
+     imp_res_tac same_ctor_and_same_tid >>
+     imp_res_tac same_tid_diff_ctor >>
+     rw [] >>
+     res_tac >>
+     fs [match_result_to_i2_def])
+ >- metis_tac []
+ >- metis_tac [length_vs_to_i2]
+ >- fs [lookup_tag_def]
  >- (every_case_tac >>
-     fs [match_result_to_i2_def, pmatch_i2_def] >>
-     rw [match_result_to_i2_def, pmatch_i2_def]
-     >- metis_tac []
+     fs [s_to_i2'_cases] >>
+     imp_res_tac store_lookup_vs_to_i2 >>
+     fs [store_lookup_def] >>
+     metis_tac [length_vs_to_i2])
+ >- (every_case_tac >>
+     fs [match_result_to_i2_def] >>
+     rw [] >>
+     pop_assum mp_tac >>
+     pop_assum mp_tac >>
+     res_tac >>
+     rw [] >>
+     CCONTR_TAC >>
+     fs [match_result_to_i2_def] >>
+     metis_tac [match_result_to_i2_def, match_result_distinct]));
 
+val (env_all_to_i2_rules, env_all_to_i2_ind, env_all_to_i2_cases) = Hol_reln `
+(!genv envC clengths lex_cenv next cenv inverse_cenv env env_i2 genv_i2.
+  cenv_inv envC (next, lex_cenv, cenv, inverse_cenv) clengths ∧
+  vs_to_i2 (cenv,clengths) genv genv_i2 ∧
+  env_to_i2 (cenv,clengths) env env_i2
+  ⇒
+  env_all_to_i2 (next, lex_cenv, cenv, inverse_cenv) (genv,envC,env) (genv_i2,env_i2) (cenv,clengths))`;
+
+val env_to_i2_append = Q.prove (
+`!cenv env1 env2 env1' env2'.
+  env_to_i2 cenv env1 env1' ∧
+  env_to_i2 cenv env2 env2' 
+  ⇒
+  env_to_i2 cenv (env1++env2) (env1'++env2')`,
+ induct_on `env1` >>
+ rw [v_to_i2_eqns] >>
+ PairCases_on `h` >>
+ fs [v_to_i2_eqns]);
+
+val env_to_i2_lookup = Q.prove (
+`!cenv env x v env'.
+  lookup x env = SOME v ∧
+  env_to_i2 cenv env env'
+  ⇒
+  ?v'.
+    v_to_i2 cenv v v' ∧
+    lookup x env' = SOME v'`,
+ induct_on `env` >>
+ rw [] >>
+ PairCases_on `h` >>
+ fs [] >>
+ cases_on `h0 = x` >>
+ fs [] >>
+ rw [] >>
+ fs [v_to_i2_eqns]);
+
+val genv_to_i2_lookup = Q.prove (
+`!cenv genv n genv'.
+  vs_to_i2 cenv genv genv' ∧
+  LENGTH genv > n
+  ⇒
+  v_to_i2 cenv (EL n genv) (EL n genv')`,
+ induct_on `genv` >>
+ srw_tac [ARITH_ss] [v_to_i2_eqns] >>
+ cases_on `n` >>
+ srw_tac [ARITH_ss] [v_to_i2_eqns]);
+
+val vs_to_i2_append1 = Q.prove (
+`!cenv vs v vs' v'.
+  vs_to_i2 cenv (vs++[v]) (vs'++[v'])
+  ⇔
+  vs_to_i2 cenv vs vs' ∧
+  v_to_i2 cenv v v'`,
+ induct_on `vs` >>
+ rw [] >>
+ cases_on `vs'` >>
+ rw [v_to_i2_eqns] 
+ >- (cases_on `vs` >>
+     rw [v_to_i2_eqns]) >>
+ metis_tac []);
+
+val do_uapp_correct = Q.prove (
+`!s uop v s' v' cenv s_i2 v_i2.
+  do_uapp_i1 s uop v = SOME (s',v') ∧
+  s_to_i2' cenv s s_i2 ∧
+  v_to_i2 cenv v v_i2
+  ⇒
+  ∃s'_i2 v'_i2.
+    s_to_i2' cenv s' s'_i2 ∧
+    v_to_i2 cenv v' v'_i2 ∧
+    do_uapp_i2 s_i2 uop v_i2 = SOME (s'_i2,v'_i2)`,
+ cases_on `uop` >>
+ rw [do_uapp_i1_def, do_uapp_i2_def, LET_THM, store_alloc_def, s_to_i2'_cases] >>
+ rw [vs_to_i2_append1, v_to_i2_eqns]
+ >- metis_tac [length_vs_to_i2] >>
+ every_case_tac >>
+ fs [v_to_i2_eqns]
+ >- metis_tac [store_lookup_vs_to_i2_2, NOT_SOME_NONE] 
+ >- metis_tac [store_lookup_vs_to_i2]);
+
+val exn_env_i2_correct = Q.prove (
+`!cenv cenv'.
+  env_all_to_i2 (next,lex_cenv,type_cenv,inverse_cenv) env env_i2 cenv'
+  ⇒
+  env_all_to_i2 (next,FST (SND init_cenv_mapping),type_cenv,inverse_cenv) (exn_env_i1 (all_env_i1_to_genv env))
+    (exn_env_i2 (all_env_i2_to_genv env_i2)) cenv'`,
+ rw [env_all_to_i2_cases, exn_env_i1_def, exn_env_i2_def, emp_def, v_to_i2_eqns,
+     all_env_i1_to_genv_def, all_env_i2_to_genv_def, init_cenv_mapping_def] >>
+ fs [cenv_inv_def, lookup_con_id_def] >>
+ rw [] >>
+ every_case_tac >>
+ fs [] >>
+ rw [id_to_n_def] >>
+ fs [has_exns_def] >>
+ fs [flookup_fupdate_list] >>
+ metis_tac []);
+
+val do_eq_i2 = Q.prove (
+`(!v1 v2 cenv r v1_i2 v2_i2 cenv'.
+  env_all_to_i2 cenv env env_i2 cenv' ∧
+  do_eq_i1 v1 v2 = r ∧
+  v_to_i2 cenv' v1 v1_i2 ∧
+  v_to_i2 cenv' v2 v2_i2
+  ⇒ 
+  do_eq_i2 v1_i2 v2_i2 = r) ∧
+ (!vs1 vs2 cenv r vs1_i2 vs2_i2 cenv'.
+  env_all_to_i2 cenv env env_i2 cenv' ∧
+  do_eq_list_i1 vs1 vs2 = r ∧
+  vs_to_i2 cenv' vs1 vs1_i2 ∧
+  vs_to_i2 cenv' vs2 vs2_i2
+  ⇒ 
+  do_eq_list_i2 vs1_i2 vs2_i2 = r)`,
+ ho_match_mp_tac do_eq_i1_ind >>
+ rw [do_eq_i2_def, do_eq_i1_def, v_to_i2_eqns] >>
+ rw [] >>
+ rw [do_eq_i2_def, do_eq_i1_def, v_to_i2_eqns] >>
+ imp_res_tac length_vs_to_i2 >>
+ fs [env_all_to_i2_cases] >>
+ rw []
+ >- metis_tac []
+ >- metis_tac []
+ >- metis_tac []
+ >- metis_tac [cenv_inv_def]
+ >- metis_tac [cenv_inv_def]
+ >- metis_tac [cenv_inv_def]
+ >- metis_tac [cenv_inv_def]
+ >- (fs [Once v_to_i2_cases] >>
+     rw [do_eq_i2_def])
+ >- (fs [Once v_to_i2_cases] >>
+     rw [do_eq_i2_def])
+ >- (fs [Once v_to_i2_cases] >>
+     rw [do_eq_i2_def])
+ >- (fs [Once v_to_i2_cases] >>
+     rw [do_eq_i2_def])
+ >- (fs [Once v_to_i2_cases] >>
+     rw [do_eq_i2_def])
+ >- (fs [Once v_to_i2_cases] >>
+     rw [do_eq_i2_def])
+ >- (fs [Once v_to_i2_cases] >>
+     rw [do_eq_i2_def])
+ >- (fs [Once v_to_i2_cases] >>
+     rw [do_eq_i2_def])
+ >- (fs [Once v_to_i2_cases] >>
+     rw [do_eq_i2_def])
+ >- (fs [Once v_to_i2_cases] >>
+     rw [do_eq_i2_def])
+ >- (fs [Once v_to_i2_cases] >>
+     rw [do_eq_i2_def])
+ >- (fs [Once v_to_i2_cases] >>
+     rw [do_eq_i2_def])
+ >- (fs [Once v_to_i2_cases] >>
+     rw [do_eq_i2_def])
+ >- (fs [Once v_to_i2_cases] >>
+     rw [do_eq_i2_def])
+ >- (fs [Once v_to_i2_cases] >>
+     rw [do_eq_i2_def])
+ >- (fs [Once v_to_i2_cases] >>
+     rw [do_eq_i2_def])
+ >- (fs [Once v_to_i2_cases] >>
+     rw [do_eq_i2_def])
+ >- (fs [Once v_to_i2_cases] >>
+     rw [do_eq_i2_def])
+ >- (fs [Once v_to_i2_cases] >>
+     rw [do_eq_i2_def])
+ >- (fs [Once v_to_i2_cases] >>
+     rw [do_eq_i2_def]) >>
+ res_tac >>
+ every_case_tac >>
+ fs [] >>
+ metis_tac []);
+
+val do_app_i2_correct = Q.prove (
+`!env s op v1 v2 s' e env' cenv s_i2 v1_i2 v2_i2 env_i2 cenv'.
+  do_app_i1 env s op v1 v2 = SOME (env',s',e) ∧
+  env_all_to_i2 cenv env env_i2 cenv' ∧
+  s_to_i2' cenv' s s_i2 ∧
+  v_to_i2 cenv' v1 v1_i2 ∧
+  v_to_i2 cenv' v2 v2_i2
+  ⇒
+  ∃s'_i2 env'_i2 cenv.
+    env_all_to_i2 cenv env' env'_i2 cenv' ∧
+    s_to_i2' cenv' s' s'_i2 ∧
+    do_app_i2 env_i2 s_i2 op v1_i2 v2_i2 = SOME (env'_i2,s'_i2,exp_to_i2 cenv e)`,
+ cases_on `op` >>
+ rw [do_app_i1_def, do_app_i2_def]
+ >- (cases_on `v2` >>
+     fs [] >>
+     cases_on `v1` >>
+     fs [v_to_i2_eqns] >>
+     rw [] >>
+     every_case_tac >>
+     fs [] >>
+     rw [] >>
+     fs [v_to_i2_eqns] >>
+     rw [exp_to_i2_def] >>
+     `?next lex_cenv type_cenv inverse_cenv. cenv = (next,lex_cenv,type_cenv,inverse_cenv)` by metis_tac [pair_CASES] >>
+     rw []
+     >- (qexists_tac `(next,FST (SND init_cenv_mapping),type_cenv,inverse_cenv)` >>
+         rw []
+         >- metis_tac [exn_env_i2_correct]
+         >- rw [init_cenv_mapping_def, flookup_fupdate_list, lookup_tag_def])
+     >- (qexists_tac `(next,FST (SND init_cenv_mapping),type_cenv,inverse_cenv)` >>
+         rw []
+         >- metis_tac [exn_env_i2_correct]
+         >- rw [init_cenv_mapping_def, flookup_fupdate_list, lookup_tag_def])
+     >- metis_tac []
+     >- metis_tac [])
+ >- (cases_on `v2` >>
+     fs [] >>
+     cases_on `v1` >>
+     fs [v_to_i2_eqns] >>
+     rw [] >>
+     every_case_tac >>
+     fs [] >>
+     rw [] >>
+     rw [exp_to_i2_def, exn_env_i2_correct] >>
+     metis_tac [])
+ >- (every_case_tac >>
+     fs [] >>
+     rw [exp_to_i2_def]
+     >- metis_tac [do_eq_i2, eq_result_11, eq_result_distinct]
+     >- metis_tac [do_eq_i2, eq_result_11, eq_result_distinct]
+     >- metis_tac [do_eq_i2, eq_result_11, eq_result_distinct]
+     >- (`?next lex_cenv type_cenv inverse_cenv. cenv = (next,lex_cenv,type_cenv,inverse_cenv)` by metis_tac [pair_CASES] >>
+         rw [] >>
+         qexists_tac `(next,FST (SND init_cenv_mapping),type_cenv,inverse_cenv)` >>
+         rw []
+         >- metis_tac [exn_env_i2_correct]
+         >- rw [init_cenv_mapping_def, flookup_fupdate_list, lookup_tag_def])
+     >- metis_tac [do_eq_i2, eq_result_11, eq_result_distinct]
+     >- metis_tac [do_eq_i2, eq_result_11, eq_result_distinct])
+ >- (every_case_tac >>
+     fs [] >>
+     pop_assum (mp_tac o SIMP_RULE (srw_ss()) [Once v_to_i2_cases]) >>
+     rw []
+     >- (qexists_tac `(next,lex_cenv,cenv'',inverse_cenv)` >>
+         rw [] >>
+         fs [env_all_to_i2_cases, bind_def] >>
+         rw [v_to_i2_eqns, all_env_i1_to_genv_def, all_env_i2_to_genv_def])
+     >- (CCONTR_TAC >>
+         fs [] >>
+         rw [] >>
+         fs [find_recfun_lookup] >>
+         induct_on `l'` >>
+         rw [] >>
+         PairCases_on `h` >>
+         fs [exp_to_i2_def] >>
+         every_case_tac >>
+         fs [])
+     >- (qexists_tac `(next,lex_cenv,cenv'',inverse_cenv)` >>
+         rw [] >>
+         fs [env_all_to_i2_cases, bind_def] >>
+         rw [v_to_i2_eqns, all_env_i1_to_genv_def, all_env_i2_to_genv_def, 
+             build_rec_env_i1_merge, build_rec_env_i2_merge, merge_def] >>
+         fs [funs_to_i2_map]
+         >- (match_mp_tac env_to_i2_append >>
+             rw [funs_to_i2_map, MAP_MAP_o, combinTheory.o_DEF, LAMBDA_PROD, env_to_i2_el,
+                 EL_MAP] >>
+             `?f x e. EL n l' = (f,x,e)` by metis_tac [pair_CASES] >>
+             rw [] >>
+             rw [Once v_to_i2_cases] >>
+             metis_tac [funs_to_i2_map])
+         >- (fs [find_recfun_lookup] >>
+             induct_on `l'` >>
+             rw [] >>
+             PairCases_on `h` >>
+             fs [exp_to_i2_def] >>
+             every_case_tac >>
+             fs [])
+         >- (fs [find_recfun_lookup] >>
+             induct_on `l'` >>
+             rw [] >>
+             PairCases_on `h` >>
+             fs [exp_to_i2_def] >>
+             every_case_tac >>
+             fs [])))
+ >- (every_case_tac >>
+     fs [] >>
+     rw [] >>
+     fs [v_to_i2_eqns, store_assign_def] 
+     >- metis_tac [length_vs_to_i2, s_to_i2'_cases] >>
+     rw [exp_to_i2_def, s_to_i2'_cases] >>
+     metis_tac [vs_to_i2_lupdate, s_to_i2'_cases]));
+
+val exp_to_i2_correct = Q.prove (
+`(∀b env s e res. 
+   evaluate_i1 b env s e res ⇒ 
+   (SND res ≠ Rerr Rtype_error) ⇒
+   !cenv s' r env_i2 s_i2 e_i2 cenv'.
+     (res = (s',r)) ∧
+     env_all_to_i2 cenv env env_i2 cenv' ∧
+     s_to_i2 cenv' s s_i2 ∧
+     (e_i2 = exp_to_i2 cenv e)
+     ⇒
+     ∃s'_i2 r_i2.
+       result_to_i2 v_to_i2 cenv' r r_i2 ∧
+       s_to_i2 cenv' s' s'_i2 ∧
+       evaluate_i2 b env_i2 s_i2 e_i2 (s'_i2, r_i2)) ∧
+ (∀b env s es res.
+   evaluate_list_i1 b env s es res ⇒ 
+   (SND res ≠ Rerr Rtype_error) ⇒
+   !cenv s' r env_i2 s_i2 es_i2 cenv'.
+     (res = (s',r)) ∧
+     env_all_to_i2 cenv env env_i2 cenv' ∧
+     s_to_i2 cenv' s s_i2 ∧
+     (es_i2 = exps_to_i2 cenv es)
+     ⇒
+     ?s'_i2 r_i2.
+       result_to_i2 vs_to_i2 cenv' r r_i2 ∧
+       s_to_i2 cenv' s' s'_i2 ∧
+       evaluate_list_i2 b env_i2 s_i2 es_i2 (s'_i2, r_i2)) ∧
+ (∀b env s v pes err_v res. 
+   evaluate_match_i1 b env s v pes err_v res ⇒ 
+   (SND res ≠ Rerr Rtype_error) ⇒
+   !cenv s' r env_i2 s_i2 v_i2 pes_i2 err_v_i2 cenv'.
+     (res = (s',r)) ∧
+     env_all_to_i2 cenv env env_i2 cenv' ∧
+     s_to_i2 cenv' s s_i2 ∧
+     v_to_i2 cenv' v v_i2 ∧
+     (pes_i2 = pat_exp_to_i2 cenv pes) ∧
+     v_to_i2 cenv' err_v err_v_i2
+     ⇒
+     ?s'_i2 r_i2.
+       result_to_i2 v_to_i2 cenv' r r_i2 ∧
+       s_to_i2 cenv' s' s'_i2 ∧
+       evaluate_match_i2 b env_i2 s_i2 v_i2 pes_i2 err_v_i2 (s'_i2, r_i2))`,
+ ho_match_mp_tac evaluate_i1_ind >>
+ rw [] >>
+ rw [Once evaluate_i2_cases,exp_to_i2_def] >>
+ TRY (Cases_on `err`) >>
+ fs [result_to_i2_eqns, v_to_i2_eqns]
+ >- metis_tac []
+ >- metis_tac []
+ >- metis_tac []
+ >- metis_tac []
+ >- metis_tac []
+ >- (* Constructor application *)
+    (res_tac >>
+     rw [] >>
+     fs [env_all_to_i2_cases, build_conv_i1_def] >>
+     rw [] >>
+     MAP_EVERY qexists_tac [`s'_i2`, `Rval (Conv_i2 (lookup_tag cn (next,lex_cenv,cenv'',inverse_cenv)) v')`] >>
+     rw [] >>
+     Cases_on `cn` >>
+     fs [] >>
+     rw [v_to_i2_eqns, lookup_tag_def] >>
+     fs [all_env_i1_to_cenv_def] >>
+     every_case_tac >>
+     fs [] >>
+     rw [v_to_i2_eqns]
+     >- metis_tac [NOT_SOME_NONE, cenv_inv_def]
+     >- metis_tac [NOT_SOME_NONE, cenv_inv_def]
+     >- metis_tac [NOT_SOME_NONE, cenv_inv_def]
+     >- metis_tac [NOT_SOME_NONE, cenv_inv_def]
+     >- (fs [cenv_inv_def, do_con_check_def] >>
+         rw [] >>
+         metis_tac [length_evaluate_list_i2, length_vs_to_i2])
+     >- metis_tac [NOT_SOME_NONE, cenv_inv_def])
+ >- metis_tac []
+ >- (* Local variable lookup *)
+    (fs [env_all_to_i2_cases, all_env_i2_to_env_def] >>
+     rw [] >>
+     fs [all_env_i1_to_env_def] >>
+     metis_tac [env_to_i2_lookup])
+ >- (* Global variable lookup *)
+    (fs [env_all_to_i2_cases, all_env_i2_to_genv_def] >>
+     rw [] >>
+     fs [all_env_i1_to_genv_def] >>
+     metis_tac [genv_to_i2_lookup, length_vs_to_i2])
+ >- (rw [Once v_to_i2_cases] >>
+     fs [env_all_to_i2_cases] >>
+     rw [all_env_i1_to_env_def, all_env_i2_to_env_def, all_env_i1_to_cenv_def] >>
+     metis_tac [])
+ >- (* Uapp *)
+    (res_tac >>
+     rw [] >>
+     fs [s_to_i2_cases] >>
+     rw [] >>
+     `?s3_i2 v'_i2. do_uapp_i2 s''' uop v'' = SOME (s3_i2, v'_i2) ∧
+       s_to_i2' cenv' s3 s3_i2 ∧ v_to_i2 cenv' v' v'_i2` by metis_tac [do_uapp_correct] >>
+     metis_tac [])
+ >- metis_tac []
+ >- (* App *)
+    (LAST_X_ASSUM (qspecl_then [`cenv`, `env_i2`, `s_i2`, `cenv'`] mp_tac) >>
+     rw [] >>
+     LAST_X_ASSUM (qspecl_then [`cenv`, `env_i2`, `s'_i2`, `cenv'`] mp_tac) >>
+     rw [] >>
+     fs [s_to_i2_cases] >>
+     rw [] >>
+     (qspecl_then [`env`, `s3`, `op`, `v1`, `v2`, `s4`, `e''`, `env'`,
+                   `cenv`, `s'''''''`, `v'`, `v''`, `env_i2`, `cenv'`] mp_tac) do_app_i2_correct >>
+     rw [] >>
+     metis_tac [])
+ >- (* App *)
+    (LAST_X_ASSUM (qspecl_then [`cenv`, `env_i2`, `s_i2`, `cenv'`] mp_tac) >>
+     rw [] >>
+     LAST_X_ASSUM (qspecl_then [`cenv`, `env_i2`, `s'_i2`, `cenv'`] mp_tac) >>
+     rw [] >>
+     fs [s_to_i2_cases] >>
+     rw [] >>
+     (qspecl_then [`env`, `s3`, `op`, `v1`, `v2`, `s4`, `e''`, `env'`,
+                   `cenv`, `s'''''''`, `v'`, `v''`, `env_i2`, `cenv'`] mp_tac) do_app_i2_correct >>
+     rw [] >>
+     metis_tac [])
+ >- (* App *)
+    (LAST_X_ASSUM (qspecl_then [`cenv`, `env_i2`, `s_i2`, `cenv'`] mp_tac) >>
+     rw [] >>
+     LAST_X_ASSUM (qspecl_then [`cenv`, `env_i2`, `s'_i2`, `cenv'`] mp_tac) >>
+     rw [] >>
+     fs [s_to_i2_cases] >>
+     rw [] >>
+     metis_tac [do_app_i2_correct])
+ >- metis_tac []
+ >- metis_tac []
+ >- metis_tac []
+ >- metis_tac []
+ >- (* If *)
+    (fs [do_if_i2_def, do_if_i1_def] >>
+     every_case_tac >>
+     rw [] >>
+     res_tac >>
+     rw [] >>
+     res_tac >>
+     rw [] >>
+     MAP_EVERY qexists_tac [`s'_i2''`, `r_i2`] >>
+     rw [] >>
+     disj1_tac
+     >- (qexists_tac `Litv_i2 (Bool F)` >>
+         fs [v_to_i2_eqns, exp_to_i2_def] >>
+         metis_tac [])
+     >- (qexists_tac `Litv_i2 (Bool T)` >>
+         fs [v_to_i2_eqns, exp_to_i2_def] >>
+         metis_tac []))
+ >- metis_tac []
+ >- metis_tac []
+ >- (* Match *)
+    (pop_assum mp_tac >>
+     res_tac >>
+     rw [] >>
+     FIRST_X_ASSUM (qspecl_then [`cenv`, `env_i2`, `s'_i2'`, `v''`, `Conv_i2 bind_tag []`, `cenv'` ] mp_tac) >>
+     rw [] >>
+     fs [env_all_to_i2_cases] >>
+     rw [] >>
+     fs [cenv_inv_def, has_exns_def] >>
+     pop_assum mp_tac >>
+     rw [] >>
+     MAP_EVERY qexists_tac [`s'_i2''`, `r_i2`] >>
+     rw [] >>
+     metis_tac [])
+ >- metis_tac []
+ >- metis_tac []
+ >- (* Let *)
+    (`?genv' env'. env_i2 = (genv',env')` by metis_tac [pair_CASES] >>
+     rw [] >>
+     res_tac >>
+     fs [] >>
+     rw [] >>
+     `env_all_to_i2 cenv' (genv,cenv,bind n v env) (genv', (n,v')::env') cenv''`
+                by (fs [env_all_to_i2_cases] >>
+                    fs [bind_def, v_to_i2_eqns] >>
+                    rw []) >>
+     metis_tac [bind_def])
+ >- metis_tac []
+ >- metis_tac []
+ >- (* Letrec *)
+    (pop_assum mp_tac >>
+     rw [] >>
+     `?genv' env'. env_i2 = (genv',env')` by metis_tac [pair_CASES] >>
+     rw [] >>
+     `env_all_to_i2 cenv' (genv,cenv,build_rec_env_i1 funs (cenv,env) env) 
+                          (genv',build_rec_env_i2 (funs_to_i2 cenv' funs) env' env') 
+                          cenv''`
+         by (fs [env_all_to_i2_cases] >>
+             rw [build_rec_env_i1_merge, build_rec_env_i2_merge, merge_def] >>
+             match_mp_tac env_to_i2_append >>
+             rw [] >>
+             rw [funs_to_i2_map, MAP_MAP_o, combinTheory.o_DEF, LAMBDA_PROD, env_to_i2_el, EL_MAP] >>
+             `?f x e. EL n funs = (f,x,e)` by metis_tac [pair_CASES] >>
+             rw [] >>
+             rw [Once v_to_i2_cases] >>
+             metis_tac [funs_to_i2_map]) >>
+      res_tac >>
+      MAP_EVERY qexists_tac [`s'_i2'`, `r_i2'`] >>
+      rw [] >>
+      disj1_tac >>
+      rw [funs_to_i2_map, MAP_MAP_o, combinTheory.o_DEF, LAMBDA_PROD])
+ >- metis_tac []
+ >- metis_tac []
+ >- metis_tac []
+ >- metis_tac []
+ >- metis_tac []
+ >- (pop_assum mp_tac >>
+     rw [] >>
+     fs [s_to_i2_cases, env_all_to_i2_cases] >>
+     rw [] >>
+     `match_result_to_i2 (cenv''',clengths) (Match env') 
+            (pmatch_i2 s'' (pat_to_i2 (next,lex_cenv,cenv''',inverse_cenv) p) v_i2 env_i2')`
+                   by metis_tac [pmatch_to_i2_correct, match_result_distinct] >>
+     cases_on `pmatch_i2 s'' (pat_to_i2 (next,lex_cenv,cenv''',inverse_cenv) p) v_i2 env_i2'` >>
+     fs [match_result_to_i2_def] >>
+     rw [] >>
+     fs [METIS_PROVE [] ``(((?x. P x) ∧ R ⇒ Q) ⇔ !x. P x ∧ R ⇒ Q) ∧ ((R ∧ (?x. P x) ⇒ Q) ⇔ !x. R ∧ P x ⇒ Q) ``] >>
+     FIRST_X_ASSUM (qspecl_then [`clengths`, `lex_cenv`, `next`, `cenv'''`, `inverse_cenv`, `a`, `genv_i2`, `s''`] mp_tac) >>
+     rw [] >>
+     fs [] >>
+     MAP_EVERY qexists_tac [`(c, s''''')`, `r_i2`] >>
+     rw [] >>
+     metis_tac [pat_bindings_to_i2])
+ >- (pop_assum mp_tac >>
+     rw [] >>
+     fs [s_to_i2_cases, env_all_to_i2_cases] >>
+     rw [] >>
+     `match_result_to_i2 (cenv''',clengths) No_match 
+            (pmatch_i2 s'' (pat_to_i2 (next,lex_cenv,cenv''',inverse_cenv) p) v_i2 env_i2')`
+                   by metis_tac [pmatch_to_i2_correct, match_result_distinct] >>
+     cases_on `pmatch_i2 s'' (pat_to_i2 (next,lex_cenv,cenv''',inverse_cenv) p) v_i2 env_i2'` >>
+     fs [match_result_to_i2_def] >>
+     rw [] >>
+     fs [METIS_PROVE [] ``(((?x. P x) ∧ R ⇒ Q) ⇔ !x. P x ∧ R ⇒ Q) ∧ ((R ∧ (?x. P x) ⇒ Q) ⇔ !x. R ∧ P x ⇒ Q) ``] >>
+     metis_tac [pat_bindings_to_i2]));
+
+val cenv_mapping_to_cenv_def = Define `
+cenv_mapping_to_cenv cenv_mapping clengths =
+   case cenv_mapping of
+     (a,b,c,d) => (c, clengths)`;
+
+     (*
+val decs_to_i2_correct = Q.prove (
+`!genv envC s1 ds r.
+  evaluate_decs_i1 genv envC s1 ds r
+  ⇒
+  !s1_i2 genv_i2 cenv_mapping ds_i2 cenv_mapping' genv' envC' s' res clengths.
+    r = (s', envC', genv', res) ∧
+    res ≠ SOME Rtype_error ∧
+    (cenv_mapping', ds_i2) = decs_to_i2 cenv_mapping ds ∧
+    cenv_inv envC cenv_mapping clengths ∧
+    s_to_i2' (cenv_mapping_to_cenv cenv_mapping clengths) s1 s1_i2 ∧
+    vs_to_i2 (cenv_mapping_to_cenv cenv_mapping clengths) genv genv_i2
+    ⇒
+    ?r_i2 genv'_i2 s'_i2 res_i2 clengths'.
+      evaluate_decs_i2 genv_i2 s1_i2 ds_i2 (s'_i2,genv'_i2,res_i2) ∧
+      cenv_inv (merge_envC (emp,envC') envC) cenv_mapping' clengths' ∧
+      vs_to_i2 (cenv_mapping_to_cenv cenv_mapping' clengths') genv' genv'_i2 ∧
+      s_to_i2' (cenv_mapping_to_cenv cenv_mapping' clengths') s' s'_i2 ∧
+      (res = NONE ∧ res_i2 = NONE ∨
+       ?err err_i2. res = SOME err ∧ res_i2 = SOME err_i2 ∧ result_to_i2 (\a b c. T) (cenv_mapping_to_cenv cenv_mapping' clengths') (Rerr err) (Rerr err_i2))`,
+      
+
+ ho_match_mp_tac evaluate_decs_i1_ind >>
+ rw [decs_to_i2_def] >>
+ every_case_tac >>
+ fs [LET_THM, evaluate_dec_i1_cases] >>
+ rw []  
+ >- (fs [emp_def, Once evaluate_decs_i2_cases, v_to_i2_eqns, s_to_i2'_cases] >>
+     PairCases_on `envC` >>
+     PairCases_on `cenv_mapping` >>
+     fs [merge_envC_def, merge_def, cenv_inv_def, cenv_mapping_to_cenv_def] >>
+     qexists_tac `clengths` >>
+     rw [] >>
+     metis_tac [])
+ >- (`?cenv_mapping' ds_i2. decs_to_i2 cenv_mapping ds = (cenv_mapping', ds_i2)` by metis_tac [pair_CASES] >>
+     fs [] >>
+     rw [Once evaluate_decs_i2_cases] >>
+     fs [s_to_i2'_cases] >>
+     `env_all_to_i2 cenv_mapping (genv,envC,emp) (genv_i2,[]) (cenv_mapping_to_cenv cenv_mapping clengths)` 
+                 by (fs [env_all_to_i2_cases, cenv_mapping_to_cenv_def] >>
+                     rw [emp_def, v_to_i2_eqns] >>
+                     every_case_tac >>
+                     metis_tac []) >>
+     imp_res_tac exp_to_i2_correct >>
+     fs [] >>
+     pop_assum mp_tac >>
+     rw [s_to_i2_cases, s_to_i2'_cases] >>
+     res_tac >>
+     fs [] >>
+     res_tac >>
+     fs [] >>
+     rw [evaluate_dec_i2_cases] >>
+     fs [result_to_i2_cases] >>
+     rw [] >>
+     cheat)
+ >- (`?cenv_mapping' ds_i2. decs_to_i2 cenv_mapping ds = (cenv_mapping', ds_i2)` by metis_tac [pair_CASES] >>
+     fs [] >>
+     rw [Once evaluate_decs_i2_cases] >>
+     fs [s_to_i2'_cases] >>
+     `env_all_to_i2 cenv_mapping (genv,envC,emp) (genv_i2,[]) (cenv_mapping_to_cenv cenv_mapping clengths)` 
+                 by (fs [env_all_to_i2_cases, cenv_mapping_to_cenv_def] >>
+                     rw [emp_def, v_to_i2_eqns] >>
+                     every_case_tac >>
+                     metis_tac []) >>
+     imp_res_tac exp_to_i2_correct >>
+     fs [] >>
+     pop_assum mp_tac >>
+     rw [s_to_i2_cases, s_to_i2'_cases] >>
+     res_tac >>
+     fs [] >>
+     res_tac >>
+     fs [] >>
+     rw [evaluate_dec_i2_cases] >>
+     fs [result_to_i2_cases, v_to_i2_eqns] >>
+     rw [] >>
+
+     metis_tac [] >>
+
+     cheat)
+
+
+
+
+val prompt_to_i2_correct = Q.prove (
+`!genv envC s prompt r.
+  evaluate_prompt_i1 genv envC s prompt r
+  ⇒
+  !s1_i2 genv_i2 cenv_mapping prompt_i2 cenv_mapping' genv' envC' s' res clengths.
+    r = (s', envC', genv', res) ∧
+    res ≠ SOME Rtype_error ∧
+    (cenv_mapping', prompt_i2) = prompt_to_i2 cenv_mapping prompt ∧
+    cenv_inv envC cenv_mapping clengths ∧
+    s_to_i2' (cenv_mapping_to_cenv cenv_mapping clengths) s s1_i2 ∧
+    vs_to_i2 (cenv_mapping_to_cenv cenv_mapping clengths) genv genv_i2
+    ⇒
+    ?genv'_i2 s'_i2 res_i2 clengths'.
+      evaluate_prompt_i2 genv_i2 s1_i2 prompt_i2 (s'_i2,genv'_i2,res_i2) ∧
+      cenv_inv (merge_envC envC' envC) cenv_mapping' clengths' ∧
+      vs_to_i2 (cenv_mapping_to_cenv cenv_mapping' clengths') genv' genv'_i2 ∧
+      s_to_i2' (cenv_mapping_to_cenv cenv_mapping' clengths') s' s'_i2 ∧
+      (res = NONE ∧ res_i2 = NONE ∨
+       ?err err_i2. res = SOME err ∧ res_i2 = SOME err_i2 ∧ result_to_i2 (\a b c. T) (cenv_mapping_to_cenv cenv_mapping' clengths') (Rerr err) (Rerr err_i2))`,
+
+ rw [evaluate_prompt_i1_cases, evaluate_prompt_i2_cases, prompt_to_i2_def] >>
+ every_case_tac >>
+ fs [LET_THM] >>
+ rw [] >>
+ `?cenv_mapping' prompt_i2. decs_to_i2 cenv_mapping ds = (cenv_mapping',prompt_i2)` by metis_tac [pair_CASES] >>
+ fs [] >>
+ rw []
+
+ *)
 val _ = export_theory ();
