compiler/intLang2Script.sml
@@ -135,8 +135,8 @@ val _ = Hol_datatype `
 val _ = Lib.with_flag (computeLib.auto_import_definitions, false) Defn.save_defn pat_bindings_i2_defn;
 
 (* The constructor names that are in scope, the global mapping of constructor
- * names (with types so that they are unique, and its inverse *)
-val _ = type_abbrev( "cenv_mapping" , ``: num # (( conN id), num) fmap # ((tid_or_exn # conN), num) fmap # (num, (tid_or_exn # conN)) fmap``);
+ * names (with types so that they are unique), and its inverse. *)
+val _ = type_abbrev( "cenv_mapping" , ``: num # (( conN id), num) fmap # ((conN # tid_or_exn), num) fmap # (num, (conN # tid_or_exn)) fmap``);
 
 (*val lookup_tag : maybe (id conN) -> cenv_mapping -> nat*)
 val _ = Define `
@@ -229,7 +229,7 @@ val _ = Lib.with_flag (computeLib.auto_import_definitions, false) Defn.save_defn
 (*val alloc_tag : maybe modN -> tid_or_exn -> conN -> cenv_mapping -> cenv_mapping*)
 val _ = Define `
  (alloc_tag mn tn cn (next, cenv,val_cenv,inv0) =
-  ((next+ 1),cenv |+ ((mk_id mn cn), next),val_cenv |+ ((tn,cn), next),inv0 |+ (next, (tn,cn))))`;
+  ((next+ 1),cenv |+ ((mk_id mn cn), next),val_cenv |+ ((cn,tn), next),inv0 |+ (next, (cn,tn))))`;
 
 
 (*val alloc_tags : maybe modN -> cenv_mapping -> type_def -> cenv_mapping*)
@@ -773,16 +773,16 @@ val _ = Define `
                  (Short "Eq", eq_tag); 
                  (Short "::", cons_tag);
                  (Short "nil", nil_tag)],
-   FUPDATE_LIST FEMPTY [((TypeExn NONE, "Div"), div_tag); 
-                 ((TypeExn NONE, "Bind"), bind_tag); 
-                 ((TypeExn NONE, "Eq"), eq_tag); 
-                 ((TypeId (Short "list"), "::"), cons_tag);
-                 ((TypeId (Short "list"), "nil"), nil_tag)],
-   FUPDATE_LIST FEMPTY [(div_tag, (TypeExn NONE, "Div")); 
-                 (bind_tag, (TypeExn NONE, "Bind")); 
-                 (eq_tag, (TypeExn NONE, "Eq")); 
-                 (cons_tag, (TypeId (Short "list"), "::"));
-                 (nil_tag, (TypeId (Short "list"), "nil"))]))`;
+   FUPDATE_LIST FEMPTY [(("Div", TypeExn NONE), div_tag); 
+                 (("Bind", TypeExn NONE), bind_tag); 
+                 (("Eq", TypeExn NONE), eq_tag); 
+                 (("::", TypeId (Short "list")), cons_tag);
+                 (("nil", TypeId (Short "list")), nil_tag)],
+   FUPDATE_LIST FEMPTY [(div_tag, ("Div", TypeExn NONE)); 
+                 (bind_tag, ("Bind", TypeExn NONE)); 
+                 (eq_tag, ("Eq", TypeExn NONE)); 
+                 (cons_tag, ("::", TypeId (Short "list")));
+                 (nil_tag, ("nil", TypeId (Short "list")))]))`;
 
 
 
